coq/lib/Relations_ext.v
@@ -1,5 +1,6 @@
 From mathcomp Require Import ssreflect ssrfun ssrbool eqtype ssrnat.
 From Coq Require Import Relations Relation_Operators.
+Export Relations Relation_Operators.
 
 Set Implicit Arguments.
 Unset Strict Implicit.
@@ -12,22 +13,25 @@ Notation "[= R ]" := [* fun x y => R x y \/ R y x ]
 
 Notation inclusion R R' := (forall t1 t2, R t1 t2 -> R' t1 t2).
 Notation same_relation R R' := (forall t1 t2, R t1 t2 <-> R' t1 t2).
+Notation wconfluent R :=
+  (forall t1 t2 t3, R t1 t2 -> R t1 t3 ->
+                    exists2 t4, [*R%type] t2 t4 & [*R%type] t3 t4).
 Notation confluent R :=
   (forall t1 t2 t3, R t1 t2 -> R t1 t3 ->
                     exists2 t4, R%type t2 t4 & R%type t3 t4).
-Notation wconfluent R :=
-  (forall t1 t2 t3, R t1 t2 -> R t1 t3 ->
-                    exists2 t4, [* R%type] t2 t4 & [* R%type] t3 t4).
+Notation church_rosser R :=
+  (forall t1 t2, [= R] t1 t2 ->
+                 exists2 t3, [*R%type] t1 t3 & [*R%type] t2 t3).
 
 Hint Resolve rt1n_refl.
 
-Lemma rtc_trans A R : transitive A [* R].
+Lemma rtc_trans A R : transitive A [*R].
 Proof. by move => t1 t2 t3; rewrite -!clos_rt_rt1n_iff; apply rt_trans. Qed.
 
-Lemma rtc_step A (R : relation A) : inclusion R [* R].
+Lemma rtc_step A (R : relation A) : inclusion R [*R].
 Proof. by move => x y H; apply rt1n_trans with y. Qed.
 
-Lemma rtc_map A (R R' : relation A) : inclusion R R' -> inclusion [* R] [* R'].
+Lemma rtc_map A (R R' : relation A) : inclusion R R' -> inclusion [*R] [*R'].
 Proof.
 move => H t t'; elim/clos_refl_trans_1n_ind: t t' / => // t1 t2 T3 H0 H1 H2.
 apply rt1n_trans with t2; auto.
@@ -35,13 +39,13 @@ Qed.
 
 Lemma rtc_map' A B (R : relation A) (R' : relation B) (f : A -> B) :
   inclusion R (fun x y => R' (f x) (f y)) ->
-  inclusion [* R] (fun x y => [* R'] (f x) (f y)).
+  inclusion [*R] (fun x y => [*R'] (f x) (f y)).
 Proof.
 move => H t t'; elim/clos_refl_trans_1n_ind: t t' / => //= x y z H0 H1 H2.
 apply rt1n_trans with (f y); auto.
 Qed.
 
-Lemma rtc_nest_elim A (R : relation A) : same_relation [* [* R]] [* R].
+Lemma rtc_nest_elim A (R : relation A) : same_relation [*[*R]] [*R].
 Proof.
 move => t1 t2; split.
 - by elim/clos_refl_trans_1n_ind: t1 t2 / => // t1 t2 t3 H _ H0;
@@ -50,10 +54,9 @@ move => t1 t2; split.
 Qed.
 
 Lemma rtc_semi_confluent' A (R R' : relation A) :
-  (forall t1 t2 t3, R t1 t2 -> R' t1 t3 ->
-    exists2 t4, R' t2 t4 & [* R] t3 t4) ->
-  (forall t1 t2 t3, [* R] t1 t2 -> R' t1 t3 ->
-    exists2 t4, R' t2 t4 & [* R] t3 t4).
+  (forall t1 t2 t3, R t1 t2 -> R' t1 t3 -> exists2 t4, R' t2 t4 & [*R] t3 t4) ->
+  (forall t1 t2 t3, [*R] t1 t2 -> R' t1 t3 ->
+    exists2 t4, R' t2 t4 & [*R] t3 t4).
 Proof.
 move => H t1 t2 t3 H0; elim/clos_refl_trans_1n_ind: t1 t2 / H0 t3.
 - by move => t1 t3 H0; exists t3.
@@ -65,36 +68,65 @@ Qed.
 
 Lemma rtc_semi_confluent A (R R' : relation A) :
   (forall t1 t2 t3, R t1 t2 -> R' t1 t3 -> exists2 t4, R' t2 t4 & R t3 t4) ->
-  (forall t1 t2 t3, [* R] t1 t2 -> R' t1 t3 ->
-    exists2 t4, R' t2 t4 & [* R] t3 t4).
+  (forall t1 t2 t3, [*R] t1 t2 -> R' t1 t3 ->
+    exists2 t4, R' t2 t4 & [*R] t3 t4).
 Proof.
 move => H; apply rtc_semi_confluent' => t1 t2 t3 H0 H1.
 by case: (H _ _ _ H0 H1) => t4 H2 H3; exists t4 => //; apply rtc_step.
 Qed.
 
-Lemma rtc_confluent A (R : relation A) : confluent R -> confluent [* R].
+Lemma rtc_confluent A (R : relation A) : confluent R -> confluent [*R].
 Proof.
 move => H; apply rtc_semi_confluent => t1 t2 t3 H0 H1.
 by case: (rtc_semi_confluent H H1 H0) => t4 H2 H3; exists t4.
 Qed.
 
 Lemma rtc_confluent' A (R R' : relation A) :
-  inclusion R R' -> inclusion R' [* R] -> confluent R' -> confluent [* R].
+  inclusion R R' -> inclusion R' [*R] -> confluent R' -> confluent [*R].
 Proof.
 move => H H0 H1 t1 t2 t3 H2 H3.
 case: (rtc_confluent H1 (rtc_map H H2) (rtc_map H H3)) => t4 H4 H5.
 by exists t4; apply rtc_nest_elim; apply (rtc_map H0).
 Qed.
 
+Lemma equiv_refl A (R : relation A) : reflexive A [= R].
+Proof. by []. Qed.
+
+Lemma equiv_trans A (R : relation A) : transitive A [= R].
+Proof. apply rtc_trans. Qed.
+
+Lemma equiv_sym A (R : relation A) : symmetric A [= R].
+Proof.
+move => x y; elim/clos_refl_trans_1n_ind: x y / => //= x y z H _ H0.
+by apply equiv_trans with y => //; apply rtc_step; case: H; auto.
+Qed.
+
+Lemma equiv_includes_rtc A (R : relation A) : inclusion [* R] [= R].
+Proof.
+move => x y; elim/clos_refl_trans_1n_ind: x y / => //= x y z H _ H0.
+by apply rt1n_trans with y => //; left.
+Qed.
+
+Lemma confluent_CR A (R : relation A) : confluent [* R] <-> church_rosser R.
+Proof.
+split; last by move => H x y z Hy Hz; apply H, equiv_trans with x;
+               [apply equiv_sym, equiv_includes_rtc | apply equiv_includes_rtc].
+move => H x y; elim/clos_refl_trans_1n_ind: x y /; first by move => x; exists x.
+move => x y z [] H0 H1 [c H2 H3].
+- by exists c => //; apply rt1n_trans with y.
+- by case: (H _ _ _ (rtc_step H0) H2) => c' H4 H5;
+    exists c' => //; apply rtc_trans with c.
+Qed.
+
 Section Z.
 
 Variable (A : Type) (R : relation A) (comp : A -> A).
-Variable (Z : forall x y, R x y -> [* R] y (comp x) /\ [* R] (comp x) (comp y)).
+Variable (Z : forall x y, R x y -> [*R] y (comp x) /\ [*R] (comp x) (comp y)).
 
-Lemma Z_confluent : confluent [* R].
+Lemma Z_confluent : confluent [*R].
 Proof.
-have Z1 x y : R x y -> [* R] y (comp x) by firstorder.
-have Z2 x y : R x y -> [* R] (comp x) (comp y) by firstorder.
+have Z1 x y : R x y -> [*R] y (comp x) by firstorder.
+have Z2 x y : R x y -> [*R] (comp x) (comp y) by firstorder.
 apply rtc_semi_confluent' => t1 t2 t3 H H0; exists (comp t3).
 - apply rtc_trans with (comp t1); first apply Z1 => //.
   apply rtc_nest_elim; move: t1 t3 H0 {H}; apply rtc_map', Z2.
@@ -108,7 +140,7 @@ Qed.
 End Z.
 
 Lemma rtc_preservation A (P : A -> Prop) (R : relation A) :
-  (forall x y, R x y -> P x -> P y) -> forall x y, [* R] x y -> P x -> P y.
+  (forall x y, R x y -> P x -> P y) -> forall x y, [*R] x y -> P x -> P y.
 Proof.
 move => H x y; elim/clos_refl_trans_1n_ind: x y / => //= x y z H0 _ H1 H2.
 exact (H1 (H x y H0 H2)).
@@ -138,7 +170,7 @@ by apply H => [x' | y'] H2; [apply IHx | apply IHy].
 Qed.
 
 Lemma Acc_wconfluent A (R : relation A) :
-  (forall x, Acc (fun a => R^~ a) x) -> wconfluent R -> confluent [* R].
+  (forall x, Acc (fun a => R^~ a) x) -> wconfluent R -> confluent [*R].
 Proof.
 move => Hacc Hwconfluent x; elim/Acc_ind': x / (Hacc x) => x IH y z Hy Hz.
 inversion Hy; subst; first by exists z.
